

:||Q2

ESTIMATIVAS INICIAIS:  $P_1: -0.586$  $P_2: 0.436$ FUNÇÃO:  $x^3 - 4x - 1$  $P_5: ?$ 

$$P_3: \frac{-0.586 \cdot f(0.436) - 0.436 \cdot f(-0.586)}{f(0.436) - f(-0.586)} = -0.278969179$$

$\nearrow -2.661118144$ 
 $\nearrow 1.142769944$

$$P_4: \frac{0.436 \cdot f(-0.278969179) - (-0.278969179) \cdot f(0.436)}{f(-0.278969179) - f(0.436)} = -0.2545339581$$

$\hookrightarrow 0.09416627362$

$$P_5: \frac{-0.278969179 \cdot f(-0.2545339581) - (-0.2545339581) \cdot f(-0.278969179)}{f(-0.2545339581) - f(-0.278969179)} = 0.001645204471$$

$\nearrow P_3$ 
 $\nearrow P_4$ 
 $\nearrow P_3$

$$= -0.2540994524$$

(C)

:11 Q1

(Aure INICIAL:  $1.911 = p_1$ ENCONTRAR  $\underline{p_5}$ :  $2.114907541 \rightarrow \textcircled{B}$ FUNÇÃO:  $x^3 - 4x - 1$ ; DERIVADA:  $3x^2 - 4$ 

$$p_2 = 1.911 - \frac{f(p_1)}{f'(p_1)} = 2.150395587$$

$$p_3 = 2.150395587 - \frac{f(p_2)}{f'(p_2)} = 2.115725962$$

$$p_4 = 2.115725962 - \frac{f(p_3)}{f'(p_3)} = 2.114907992$$

$$p_5 = 2.114907992 - \frac{f(p_4)}{f'(p_4)} = \underline{\underline{2.114907541}}$$

 $\textcircled{B}$